src/program_logic/na_crash_inv.v
@@ -19,94 +19,60 @@ Implicit Types Φc : iProp Σ.
 Implicit Types v : val Λ.
 Implicit Types e : expr Λ.
 
-Definition na_crash_inv_def Γ N k :=
-  (staged_inv Γ N k (⊤ ∖ ↑N) (⊤ ∖ ↑N))%I.
+Definition na_crash_inv_def N k Q P :=
+  (∃ Γ Qr bset, staged_inv Γ N k (⊤ ∖ ↑N) (⊤ ∖ ↑N) ∗ staged_bundle Γ Q Qr false bset ∗
+                staged_crash Γ P bset)%I.
 Definition na_crash_inv_aux : seal (@na_crash_inv_def). by eexists. Qed.
 Definition na_crash_inv := (na_crash_inv_aux).(unseal).
 Definition na_crash_inv_eq := (na_crash_inv_aux).(seal_eq).
 
-Definition na_crash_bundle_def Γ N k Q bset :=
-  (∃ Qr, staged_inv Γ N k (⊤ ∖ ↑N) (⊤ ∖ ↑N) ∗ staged_bundle Γ Q Qr false bset)%I.
-Definition na_crash_bundle_aux : seal (@na_crash_bundle_def). by eexists. Qed.
-Definition na_crash_bundle := (na_crash_bundle_aux).(unseal).
-Definition na_crash_bundle_eq := (na_crash_bundle_aux).(seal_eq).
-
-Definition na_crash_val_def Γ P bset :=
-  (staged_crash Γ P bset)%I.
-Definition na_crash_val_aux : seal (@na_crash_val_def). by eexists. Qed.
-Definition na_crash_val := (na_crash_val_aux).(unseal).
-Definition na_crash_val_eq := (na_crash_val_aux).(seal_eq).
-
-Definition na_crash_pending_def Γ N k P :=
-  (∃ i, staged_inv Γ N k (⊤ ∖ ↑N) (⊤ ∖ ↑N) ∗ staged_crash_pending Γ P i)%I.
-Definition na_crash_pending_aux : seal (@na_crash_pending_def). by eexists. Qed.
-Definition na_crash_pending := (na_crash_pending_aux).(unseal).
-Definition na_crash_pending_eq := (na_crash_pending_aux).(seal_eq).
-
 Ltac crash_unseal :=
-  rewrite /na_crash_inv/na_crash_val/na_crash_pending/na_crash_bundle;
-  rewrite ?na_crash_inv_eq ?na_crash_val_eq ?na_crash_pending_eq ?na_crash_bundle_eq;
-  rewrite /na_crash_inv_def/na_crash_val_def/na_crash_pending_def/na_crash_bundle_def.
+  rewrite /na_crash_inv;
+  rewrite ?na_crash_inv_eq;
+  rewrite /na_crash_inv_def.
 
-Global Instance na_crash_inv_pers Γ N k : Persistent (na_crash_inv Γ N k).
-Proof. crash_unseal. apply _. Qed.
-
-Global Instance na_crash_val_pers Γ P bset : Persistent (na_crash_val Γ P bset).
-Proof. crash_unseal. apply _. Qed.
-
-
-Lemma na_crash_inv_init N k E:
-  ⊢ |={E}=> ∃ Γ, na_crash_inv Γ N k.
-Proof. crash_unseal. iMod (staged_inv_init) as (Γ) "H". iExists Γ. iFrame "H". eauto. Qed.
-
-Lemma na_crash_inv_alloc Γ N k E P Q:
+Lemma na_crash_inv_alloc N k E P Q:
   ↑N ⊆ E →
-  na_crash_inv Γ N k -∗
-  ▷ Q -∗ ▷ □ (Q -∗ P) ={E}=∗
-  ∃ i, na_crash_bundle Γ N k Q {[i]} ∗ na_crash_val Γ P {[i]} ∗ na_crash_pending Γ N k P.
+  ▷ Q -∗ ▷ □ (Q -∗ P) ={E}=∗ na_crash_inv N (LVL k) Q P ∗ |C={⊤, ∅}_(LVL (S k))=> P.
 Proof.
   crash_unseal.
-  iIntros (?) "#Hinv HQ #HQP".
-  iMod (staged_inv_alloc Γ N k E (⊤ ∖ ↑N) P Q True%I with "[HQ]") as (i') "(Hbundle&#Hval&Hpend)".
+  iIntros (?) "HQ #HQP".
+  iMod (staged_inv_init) as (Γ) "#H".
+  iMod (staged_inv_alloc Γ N (LVL k) E (⊤ ∖ ↑N) P Q True%I with "[HQ]") as (i') "(Hbundle&#Hval&Hpend)".
   { auto. }
   { iFrame "#". iFrame. iAlways; iIntros; eauto. iSplitL; last done.
     iApply "HQP"; eauto. }
-  iModIntro. iExists i'. iFrame "#".
+  iModIntro.
   iSplitL "Hbundle".
-  - iExists _. iFrame.
-  - iExists _. eauto.
+  { iExists _, _, _. iFrame. iFrame "#". }
+  iApply (staged_inv_init_cfupd with "[$]"); eauto.
 Qed.
 
-Lemma na_crash_inv_pending_weaken Γ N k P:
-  na_crash_pending Γ N k P -∗ na_crash_inv Γ N k.
-Proof. crash_unseal. iIntros "H". iDestruct "H" as (?) "(?&?)"; eauto. Qed.
-
-Lemma na_crash_bundle_weaken Γ N k Q Q' bset :
+Lemma na_crash_inv_weaken N k Q Q' P :
   □(Q -∗ Q') -∗
-  na_crash_bundle Γ N k Q bset -∗
-  na_crash_bundle Γ N k Q' bset.
+  na_crash_inv N k Q P -∗
+  na_crash_inv N k Q' P.
 Proof.
   crash_unseal.
   iIntros "#HQ' H".
-  iDestruct "H" as (Qr) "[Hinv Hbundle]".
-  iExists Qr; iFrame.
+  iDestruct "H" as (? Qr ?) "(Hinv&Hbundle&?)".
+  iExists _, Qr, _. iFrame.
   iApply (staged_bundle_weaken_1 with "HQ' Hbundle").
 Qed.
 
-Lemma wpc_na_crash_inv_open_modify Γ Qnew s k k' E1 E2 e Φ Φc Q P bset N :
+Lemma wpc_na_crash_inv_open_modify Qnew s k k' E1 E2 e Φ Φc Q P N :
   ↑N ⊆ E1 →
   S k < k' →
   to_val e = None →
-  na_crash_bundle Γ N (LVL k') Q bset -∗
-  na_crash_val Γ P bset -∗
+  na_crash_inv N (LVL k') Q P -∗
   (Φc ∧ (Q -∗ WPC e @ NotStuck; (LVL k); (E1 ∖ ↑N); ∅
-                    {{λ v, ▷ Qnew v ∗ ▷ □ (Qnew v -∗ P)  ∗ (na_crash_bundle Γ N (LVL k') (Qnew v) bset -∗ (Φc ∧ Φ v))}}
+                    {{λ v, ▷ Qnew v ∗ ▷ □ (Qnew v -∗ P)  ∗ (na_crash_inv N (LVL k') (Qnew v) P -∗ (Φc ∧ Φ v))}}
                     {{ Φc ∗ ▷ P }})) -∗
   WPC e @ s; LVL (S k); E1; E2 {{ Φ }} {{ Φc }}.
 Proof.
   crash_unseal.
-  iIntros (???) "Hbundle Hval Hwp".
-  iDestruct "Hbundle" as (?) "(#Hinv&Hbundle)".
+  iIntros (???) "Hbundle Hwp".
+  iDestruct "Hbundle" as (???) "(#Hinv&Hbundle&#Hval)".
   iApply (wpc_staged_inv_open _ _ _ _ _ _ _ _ _ _ _ _ Qnew); eauto.
   iFrame "Hinv". iFrame "Hval". iFrame "Hbundle".
   iSplit.
@@ -116,110 +82,59 @@ Proof.
   iApply (wpc_strong_mono' with "Hwp"); eauto.
   iSplit.
   - iIntros (?) "(HQ&#Hwand'&HQrest)".
-    iModIntro. iFrame "HQ Hwand'". iIntros "Hval".
-    iApply "HQrest". iFrame. iFrame "Hinv". iExists _. iFrame.
+    iModIntro. iFrame "HQ Hwand'". iIntros "Hval'".
+    iApply "HQrest". iFrame. iExists _, _, _. iFrame "∗ #".
   - iIntros. rewrite difference_diag_L. iModIntro; eauto.
 Qed.
 
-Lemma wpc_na_crash_inv_open Γ s k k' E1 E2 e Φ Φc Q P bset N:
+Lemma wpc_na_crash_inv_open s k k' E1 E2 e Φ Φc Q P N:
   ↑N ⊆ E1 →
   S k < k' →
   to_val e = None →
-  na_crash_bundle Γ N (LVL k') Q bset -∗
-  na_crash_val Γ P bset -∗
+  na_crash_inv N (LVL k') Q P -∗
   (Φc ∧ (Q -∗ WPC e @ NotStuck; (LVL k); (E1 ∖ ↑N); ∅
-                    {{λ v, ▷ Q ∗ ▷ □ (Q -∗ P) ∗ (na_crash_bundle Γ N (LVL k') Q bset -∗ (Φc ∧ Φ v))}}
+                    {{λ v, ▷ Q ∗ ▷ □ (Q -∗ P) ∗ (na_crash_inv N (LVL k') Q P -∗ (Φc ∧ Φ v))}}
                     {{ Φc ∗ ▷ P }})) -∗
   WPC e @ s; LVL (S k); E1; E2 {{ Φ }} {{ Φc }}.
 Proof.
-  iIntros (???) "H1 H2 Hwp". iApply (wpc_na_crash_inv_open_modify with "[$] [$]"); auto.
+  iIntros (???) "H1 Hwp". iApply (wpc_na_crash_inv_open_modify with "[$] [$]"); auto.
 Qed.
 
-Lemma wpc_na_crash_inv_init Γ s k k' N E2 e Φ Φc P :
-  k' < k →
-  na_crash_pending Γ N (LVL k') P ∗
-  WPC e @ s; LVL k; ⊤; E2 {{ Φ }} {{ Φc }} ⊢
-  WPC e @ s; LVL (S k); ⊤; E2 {{ Φ }} {{ Φc ∗ P }}.
-Proof.
-  crash_unseal.
-  iIntros (?) "(H&?)".
-  iDestruct "H" as (?) "(?&?)".
-  iApply wpc_staged_inv_init; last (by iFrame); eauto.
-Qed.
-
-Lemma wpc_na_crash_inv_init_wand Γ s k k' N E2 e Φ Φc P :
-  k' < k →
-  na_crash_pending Γ N (LVL k') P -∗
-  WPC e @ s; LVL k; ⊤; E2 {{ Φ }} {{ P -∗ Φc }} -∗
-  WPC e @ s; LVL (S k); ⊤; E2 {{ Φ }} {{ Φc }}.
-Proof.
-  crash_unseal.
-  iIntros (?) "H ?".
-  iDestruct "H" as (?) "(?&?)".
-  iApply wpc_staged_inv_init_wand; last (by iFrame); eauto.
-Qed.
-
-Lemma wpc_na_crash_inv_big_sepS_init_wand `{Countable A} (σ: gset A)(P: A → iProp Σ) k s E2 e Φ Φc  :
-  ([∗ set] a ∈ σ, ∃ Γ N k', ⌜ k' < k ⌝ ∗ na_crash_pending Γ N (LVL k') (P a)) -∗
-  WPC e @ s; LVL k; ⊤; E2 {{ Φ }} {{ ([∗ set] a ∈ σ, P a) -∗ Φc }} -∗
-  WPC e @ s; LVL (k + size σ); ⊤; E2 {{ Φ }} {{ Φc }}.
-Proof.
-  iInduction σ as [| x σ ?] "IH" using set_ind_L forall (Φc).
-  - rewrite size_empty right_id. iIntros "_ Hwp".
-    iApply (wpc_mono with "Hwp"); eauto.
-    rewrite big_sepS_empty //=. iIntros "H". by iApply "H".
-  - rewrite big_sepS_union; last by set_solver.
-    rewrite big_sepS_singleton.
-    iIntros "(HPx&Hrest)". iDestruct "HPx" as (?? k' Hlt) "Hpending".
-    iIntros "Hwp". replace (k + size ({[x]} ∪ σ)) with (S (k + size σ)); last first.
-    { rewrite size_union; last by set_solver. rewrite size_singleton. lia. }
-    iApply (wpc_na_crash_inv_init_wand with "Hpending").
-    { lia. }
-    iApply ("IH" with "Hrest").
-    iApply (wpc_mono with "Hwp"); auto.
-    iIntros "Hwand Hrest HP". iApply "Hwand".
-    rewrite big_sepS_union ?big_sepS_singleton; last by set_solver.
-    iFrame.
-Qed.
-
-Lemma na_crash_inv_open_modify Γ N k' k E E' P Q R bset:
+Lemma na_crash_inv_open_modify N k' k E E' P Q R:
   ↑N ⊆ E →
-  na_crash_bundle Γ N k' Q bset -∗
-  na_crash_val Γ P bset -∗
-  ((Q ∗ (∀ Q', ▷ Q' ∗ □ (Q' -∗ P) ={E∖↑N,E}=∗ na_crash_bundle Γ N k' Q' bset)) ∨ (C ∗ |={E∖↑N, E}=> na_crash_bundle Γ N k' Q bset)
+  na_crash_inv N k' Q P -∗
+  ((Q ∗ (∀ Q', ▷ Q' ∗ □ (Q' -∗ P) ={E∖↑N,E}=∗ na_crash_inv N k' Q' P)) ∨ (C ∗ |={E∖↑N, E}=> na_crash_inv N k' Q P)
    -∗ |={E ∖ ↑N, E'}_k=> R) -∗
   (|={E,E'}_(S (S k))=> R).
 Proof.
   crash_unseal.
   iIntros (?) "Hbundle Hwp".
-  iDestruct "Hbundle" as (?) "(#Hinv&Hbundle)".
+  iDestruct "Hbundle" as (???) "(#Hinv&Hbundle&#Hval)".
   iMod (staged_inv_open with "[$]") as "HQ"; auto.
   iMod (fupd_intro_mask' _ ∅) as "Hclo"; first set_solver.
-  iIntros "H".
   iModIntro.
   rewrite Nat_iter_S.
   iModIntro. iNext. iModIntro.
   rewrite Nat_iter_S.
   iModIntro. iNext. iMod "Hclo" as "_".
-  iApply ("H" with "[HQ]").
+  iApply ("Hwp" with "[HQ]").
   iDestruct "HQ" as "[(HQ&Hclo)|(?&HC&Hclo)]".
   - iLeft. iFrame. iIntros (Q') "(HQ'&#Hwand')". iMod ("Hclo" $! Q' True%I false with "[HQ']") as "H".
     { iFrame. iAlways. iIntros. iSplitL; last done. by iApply "Hwand'". }
-    iModIntro. iExists _. iFrame "H Hinv Hwand'".
-  - iRight. iFrame. iMod "Hclo". iModIntro. iExists _. iFrame. iFrame "#".
+    iModIntro. iExists _, _, _. iFrame "# ∗".
+  - iRight. iFrame. iMod "Hclo". iModIntro. iExists _, _, _. iFrame "# ∗".
 Qed.
 
-Lemma na_crash_inv_open Γ N k' k E E' P Q R bset:
+Lemma na_crash_inv_open N k' k E E' P Q R:
   ↑N ⊆ E →
-  na_crash_bundle Γ N k' Q bset -∗
-  na_crash_val Γ P bset -∗
-  ((Q ∗ (▷ Q ∗ □ (Q -∗ P) ={E∖↑N,E}=∗ na_crash_bundle Γ N k' Q bset)) ∨ (C ∗ |={E∖↑N, E}=> na_crash_bundle Γ N k' Q bset)
+  na_crash_inv N k' Q P -∗
+  ((Q ∗ (▷ Q ∗ □ (Q -∗ P) ={E∖↑N,E}=∗ na_crash_inv N k' Q P)) ∨ (C ∗ |={E∖↑N, E}=> na_crash_inv N k' Q P)
    -∗ |={E ∖ ↑N, E'}_k=> R) -∗
   (|={E,E'}_(S (S k))=> R).
 Proof.
-  iIntros (?) "H1 H2 H3".
-  iApply (na_crash_inv_open_modify with "[$] [$]"); auto.
-  iIntros "H". iApply ("H3" with "[H]").
+  iIntros (?) "H1 H2".
+  iApply (na_crash_inv_open_modify with "[$]"); auto.
+  iIntros "H". iApply ("H2" with "[H]").
   iDestruct "H" as "[H1|H2]".
    - iLeft. iDestruct "H1" as "($&H)". iIntros "HQ". by iMod ("H" $! Q with "[$]").
    - iRight. iFrame.
